Label.v
@@ -1,9 +1,0 @@
-Definition Location := nat.
-Definition Value := nat.
-
-Class LabelClass (L : Type): Type := {
-  lab_loc : L -> Location;
-  lab_val : L -> Value; 
-  is_r : L -> Prop;
-  is_w : L -> Prop;
-}. 
