Arm.v
@@ -1,0 +1,46 @@
+From RelAcqProof Require Import Events. 
+From RelAcqProof Require Import Executions. 
+From hahn Require Import Hahn.
+
+Inductive LabelArm := 
+| W_Rel (loc:Location) (val:Value)
+| R_Acq_Pc (loc:Location) (val:Value). 
+
+(* Instance LabelClassArm: LabelClass LabelArm.  *)
+Instance LabelClassArm: LabelClass LabelArm := {
+    lab_loc l := match l with
+                | W_Rel loc _ => loc 
+                | R_Acq_Pc loc _ => loc 
+                end;
+      
+    lab_val l := match l with
+                | W_Rel _ val => val 
+                | R_Acq_Pc _ val => val 
+                end;
+
+    is_r l := match l with
+                | W_Rel _ _ => False 
+                | R_Acq_Pc _ _ => True 
+                end;
+
+    is_w l := match l with
+                | W_Rel _ _ => True 
+                | R_Acq_Pc _ _ => False 
+                end;
+}. 
+
+
+(* ARM axiom *)
+(* bob = ((R_acq_pc ; po) ∪ (po ; W_rel)) *)
+Definition bob_arm {Label: Type} {LabelProof : LabelClass Label} (exec: Execution): relation Event :=
+    let R := ⦗fun r => is_r (event_label r)⦘ in 
+    let W := ⦗fun w => is_w (event_label w)⦘ in
+    (R ⨾ (po exec)) ∪ ((po exec) ⨾ W).
+
+(* ob = (bob ∪ rfe ∪ moe ∪ fre)+ *)
+Definition ordered_before_axiom_arm {Label: Type} {LabelProof : LabelClass Label} (exec: Execution): Prop :=
+    irreflexive (((bob_arm exec) ∪ (external rf exec) ∪ (external mo exec) ∪ (external fr exec))⁺).
+    
+
+Definition arm_consistent  {Label: Type} {LabelProof : LabelClass Label} (exec: Execution): Prop := 
+    well_formed exec /\ atomicity_axiom exec /\ coherence_axiom exec /\ ordered_before_axiom_arm exec. 
