X86.v
@@ -1,0 +1,51 @@
+From RelAcqProof Require Import Events. 
+From RelAcqProof Require Import Executions. 
+From hahn Require Import Hahn.
+
+Inductive LabelX86 := 
+| W_x86 (loc:Location) (val:Value)
+| R_x86 (loc:Location) (val:Value). 
+
+(* Instance LabelClassArm: LabelClass LabelArm.  *)
+Instance LabelClassX86: LabelClass LabelX86 := {
+    lab_loc l := match l with
+                | W_x86 loc _ => loc 
+                | R_x86 loc _ => loc 
+                end;
+      
+    lab_val l := match l with
+                | W_x86 _ val => val 
+                | R_x86 _ val => val 
+                end;
+
+    is_r l := match l with
+                | W_x86 _ _ => False  
+                | R_x86 _ _ => True 
+                end;
+
+    is_w l := match l with
+                | W_x86 _ _ => True  
+                | R_x86 _ _ => False
+                end;
+}. 
+
+(* atomic ops (in domain or codomain of rmw) act as a barrier between them and what happens before or after *)
+Definition implid_x86 {Label: Type} {LabelProof : LabelClass Label} (exec: Execution): relation Event :=
+    let atomic := ⦗dom_rel (rmw exec)⦘ ∪ ⦗codom_rel (rmw exec)⦘ in
+        ((po exec) ⨾ atomic) ∪ (atomic ⨾ (po exec)).
+
+(* TSO enforces everything but W -> R to be ordered *)
+(* is the last case even needed, considering we're esentially doing set difference? *)
+Definition ppo_x86 {Label: Type} {LabelProof : LabelClass Label} (exec: Execution): relation Event :=
+    (po exec) \ (fun w r => is_w (event_label w) /\ is_r (event_label r) /\ ((po exec) r w)). 
+
+(* happens before is defined by the union of several relations *)
+Definition hb_x86 {Label: Type} {LabelProof : LabelClass Label} (exec: Execution): relation Event :=
+    (ppo_x86 exec) ∪ (implid_x86 exec) ∪ (external rf exec) ∪ (fr exec) ∪ (mo exec).
+
+(* x86 Axiom: the transitive closure of happens before must be irreflexive (cycles cause it to be reflexive) *)
+Definition ordered_before_axiom_x86 {Label: Type} {LabelProof : LabelClass Label} (exec: Execution): Prop :=
+    irreflexive ((hb_x86 exec)⁺).
+
+Definition x86_consistent  {Label: Type} {LabelProof : LabelClass Label} (exec: Execution): Prop := 
+    well_formed exec /\ atomicity_axiom exec /\ coherence_axiom exec /\ ordered_before_axiom_x86 exec.
